Connecting: proved an invariant for a compilation result

Connecting.v
@@ -3,13 +3,11 @@
   * Author: Adam Chlipala
   * License: https://creativecommons.org/licenses/by-nc-nd/4.0/ *)
 
-Require Import FrapWithoutSets SepCancel.
-Require Import Arith.Div2.
+Require Import Frap SepCancel ModelCheck Classes.Morphisms.
+Require Import Arith.Div2 Eqdep.
 
 
 (** * Some odds and ends from past chapters *)
-
-Notation "m $! k" := (match m $? k with Some n => n | None => O end) (at level 30).
 
 Ltac simp := repeat (simplify; subst; propositional;
                      try match goal with
@@ -94,9 +92,9 @@ Hint Resolve shatter_word_0.
 
 Require Import Coq.Logic.Eqdep_dec.
 
-Definition weq : forall {sz} (x y : word sz), {x = y} + {x <> y}.
-  refine (fix weq sz (x : word sz) : forall y : word sz, {x = y} + {x <> y} :=
-    match x in word sz return forall y : word sz, {x = y} + {x <> y} with
+Definition weq : forall {sz} (x y : word sz), sumbool (x = y) (x <> y).
+  refine (fix weq sz (x : word sz) : forall y : word sz, sumbool (x = y) (x <> y) :=
+    match x in word sz return forall y : word sz, sumbool (x = y) (x <> y) with
       | WO => fun _ => left _ _
       | WS b x' => fun y => if bool_dec b (whd y)
         then if weq _ x' (wtl y) then left _ _ else right _ _
@@ -113,199 +111,144 @@ Definition weq : forall {sz} (x y : word sz), {x = y} + {x <> y}.
   abstract (rewrite (shatter_word y); simpl; intro; apply n0; injection H; auto).
 Defined.
 
+Lemma mod2_2times : forall n,
+    mod2 (2 * n) = false.
+Proof.
+  induct n; simplify; auto.
+  replace (n + S (n + 0)) with (S (2 * n)) by linear_arithmetic.
+  assumption.
+Qed.
 
-(** * A simple C-like language with just two data types *)
+Lemma mod2_plus1_2times : forall n,
+    mod2 (1 + 2 * n) = true.
+Proof.
+  induct n; simplify; auto.
+  replace (n + S (n + 0)) with (S (2 * n)) by linear_arithmetic.
+  assumption.
+Qed.
+
+Theorem adding_one_changes : forall sz (w : word sz),
+    sz > 0
+    -> w ^+ ^1 <> w.
+Proof.
+  propositional.
+  cases sz; try linear_arithmetic.
+  pose proof (shatter_word_S w); first_order; subst.
+  unfold wplus in H0.
+  simplify.
+  invert H0.
+  clear H3.
+  cases x.
+  replace (S (wordToNat x0 + (wordToNat x0 + 0)) + S (wordToNat (^ 0) + (wordToNat (^ 0) + 0)))
+          with (2 * (1 + wordToNat x0 + @wordToNat sz (^0))) in H2 by linear_arithmetic.
+  rewrite mod2_2times in H2; equality.
+  replace (wordToNat x0 + (wordToNat x0 + 0) + S (wordToNat (^ 0) + (wordToNat (^ 0) + 0)))
+          with (1 + 2 * (wordToNat x0 + @wordToNat sz (^0))) in H2 by linear_arithmetic.
+  rewrite mod2_plus1_2times in H2.
+  equality.
+Qed.
 
 Module Type BIT_WIDTH.
   Parameter bit_width : nat.
+  Axiom bit_width_nonzero : bit_width > 0.
 End BIT_WIDTH.
 
-Module DeeplyEmbedded(Import BW : BIT_WIDTH).
+
+(** * A modification of last chapter's language, to use words instead of naturals *)
+
+
+Module MixedEmbedded(Import BW : BIT_WIDTH).
   Definition wrd := word bit_width.
+  Definition heap := fmap wrd wrd.
 
-  Inductive exp :=
-  | Var (x : var)
-
-  | Const (n : wrd)
-  | Add (x : var) (n : wrd)
-
-  | Head (x : var)
-  | Tail (x : var)
-
-  | NotNull (x : var).
-
-  Inductive stmt :=
-  | Skip
-  | Assign (x : var) (e : exp)
-  | WriteHead (x : var) (e : exp)
-  | WriteTail (x : var) (e : exp)
-  | Seq (s1 s2 : stmt)
-  | IfThenElse (e : exp) (s1 s2 : stmt)
-  | WhileLoop (e : exp) (s1 : stmt).
-
-  Inductive type :=
-  | Scalar
-  | ListPointer (t : type).
-
-  Definition type_eq : forall t1 t2 : type, {t1 = t2} + {t1 <> t2}.
-    decide equality.
-  Defined.
-
-  Record function := {
-    Params : list (var * type);
-    Locals : list (var * type);
-    Return : type;
-    Body : stmt
-  }.
-
-  Section fn.
-    Variable fn : function.
-
-    Definition vars := Params fn ++ Locals fn ++ [("result", Return fn)].
-
-    Fixpoint varType (x : var) (vs : list (var * type)) : option type :=
-      match vs with
-      | nil => None
-      | (y, t) :: vs' => if y ==v x then Some t else varType x vs'
-      end.
-
-    Fixpoint expType (e : exp) : option type :=
-      match e with
-      | Var x => varType x vars
-      | Const _ => Some Scalar
-      | Add x _ => match varType x vars with
-                   | Some Scalar => Some Scalar
-                   | _ => None
-                   end
-      | Head x => match varType x vars with
-                  | Some (ListPointer t) => Some t
-                  | _ => None
-                  end
-      | Tail x => match varType x vars with
-                  | Some (ListPointer t) => Some (ListPointer t)
-                  | _ => None
-                  end
-      | NotNull x => match varType x vars with
-                     | Some (ListPointer _) => Some Scalar
-                     | _ => None
-                     end
-      end.
-
-    Fixpoint stmtWf (s : stmt) : bool :=
-      match s with
-      | Skip => true
-      | Assign x e => match varType x vars, expType e with
-                      | Some t1, Some t2 =>
-                        if type_eq t1 t2 then true else false
-                      | _, _ => false
-                      end
-      | WriteHead x e => match varType x vars, expType e with
-                         | Some (ListPointer t1), Some t2 =>
-                           if type_eq t1 t2 then true else false
-                         | _, _ => false
-                         end
-      | WriteTail x e => match varType x vars, expType e with
-                         | Some (ListPointer t1), Some (ListPointer t2) =>
-                           if type_eq t1 t2 then true else false
-                         | _, _ => false
-                         end
-      | Seq s1 s2 => stmtWf s1 && stmtWf s2
-      | IfThenElse e s1 s2 => match expType e with
-                              | Some Scalar => stmtWf s1 && stmtWf s2
-                              | _ => false
-                              end
-      | WhileLoop e s1 => match expType e with
-                          | Some Scalar => stmtWf s1
-                          | _ => false
-                          end
-      end.
-
-    Record functionWf : Prop := {
-      VarsOk : NoDup (map fst (Params fn ++ Locals fn));
-      BodyOk : stmtWf (Body fn) = true
-    }.
-  End fn.
-
-  Inductive value :=
-  | VScalar (n : wrd)
-  | VList (p : wrd).
-
-  Definition heap := fmap (wrd) (value * value).
-  Definition valuation := fmap var value.
-
-  Inductive eval : heap -> valuation -> exp -> value -> Prop :=
-  | VVar : forall H V x v,
-      V $? x = Some v
-      -> eval H V (Var x) v
-  | VConst : forall H V n,
-      eval H V (Const n) (VScalar n)
-  | VAdd : forall H V x n xn,
-      V $? x = Some (VScalar xn)
-      -> eval H V (Add x n) (VScalar (xn ^+ n))
-  | VHead : forall H V x p ph pt,
-      V $? x = Some (VList p)
-      -> H $? p = Some (ph, pt)
-      -> eval H V (Head x) ph
-  | VTail : forall H V x p ph pt,
-      V $? x = Some (VList p)
-      -> H $? p = Some (ph, pt)
-      -> eval H V (Tail x) pt
-  | VNotNull : forall H V x p,
-      V $? x = Some (VList p)
-      -> eval H V (NotNull x) (VScalar (if weq p (^0) then ^1 else ^0)).
-
-  Inductive step : heap * valuation * stmt -> heap * valuation * stmt -> Prop :=
-  | StAssign : forall H V x e v,
-      eval H V e v
-      -> step (H, V, Assign x e) (H, V $+ (x, v), Skip)
-  | StWriteHead : forall H V x e a v hv tv,
-      V $? x = Some (VList a)
-      -> eval H V e v
-      -> H $? a = Some (hv, tv)
-      -> step (H, V, WriteHead x e) (H $+ (a, (v, tv)), V, Skip)
-  | StWriteTail : forall H V x e a v hv tv,
-      V $? x = Some (VList a)
-      -> eval H V e v
-      -> H $? a = Some (hv, tv)
-      -> step (H, V, WriteTail x e) (H $+ (a, (hv, v)), V, Skip)
-  | StSeq1 : forall H V s2,
-      step (H, V, Seq Skip s2) (H, V, s2)
-  | StSeq2 : forall H V s1 s2 H' V' s1',
-      step (H, V, s1) (H', V', s1')
-      -> step (H, V, Seq s1 s2) (H', V', Seq s1' s2)
-  | StIfThen : forall H V e s1 s2 n,
-      eval H V e (VScalar n)
-      -> n <> ^0
-      -> step (H, V, IfThenElse e s1 s2) (H, V, s1)
-  | StIfElse : forall H V e s1 s2,
-      eval H V e (VScalar (^0))
-      -> step (H, V, IfThenElse e s1 s2) (H, V, s2)
-  | StWhileTrue : forall H V e s1 n,
-      eval H V e (VScalar n)
-      -> n <> ^0
-      -> step (H, V, WhileLoop e s1) (H, V, Seq s1 (WhileLoop e s1))
-  | StWhileFalse : forall H V e s1,
-      eval H V e (VScalar (^0))
-      -> step (H, V, WhileLoop e s1) (H, V, Skip).
+  Ltac simp := repeat (simplify; subst; propositional;
+                       try match goal with
+                           | [ H : ex _ |- _ ] => invert H
+                           end).
 
 
-  (** * Separation logic for our language *)
+  Inductive loop_outcome {acc} :=
+  | Done (a : acc)
+  | Again (a : acc).
 
+  Arguments loop_outcome : clear implicits.
+
+  Inductive cmd : Set -> Type :=
+  | Return {result : Set} (r : result) : cmd result
+  | Bind {result result'} (c1 : cmd result') (c2 : result' -> cmd result) : cmd result
+  | Read (a : wrd) : cmd wrd
+  | Write (a v : wrd) : cmd unit
+  | Loop {acc : Set} (init : acc) (body : acc -> cmd (loop_outcome acc)) : cmd acc
+  | Fail {result} : cmd result.
+
+  (* We're leaving out allocation and deallocation, to avoid distraction from
+   * the main point of the examples to follow. *)
+
+  Notation "x <- c1 ; c2" := (Bind c1 (fun x => c2)) (right associativity, at level 80).
+  Notation "'for' x := i 'loop' c1 'done'" := (Loop i (fun x => c1)) (right associativity, at level 80).
+
+  Inductive step : forall {A}, heap * cmd A -> heap * cmd A -> Prop :=
+  | StepBindRecur : forall result result' (c1 c1' : cmd result') (c2 : result' -> cmd result) h h',
+    step (h, c1) (h', c1')
+    -> step (h, Bind c1 c2) (h', Bind c1' c2)
+  | StepBindProceed : forall (result result' : Set) (v : result') (c2 : result' -> cmd result) h,
+    step (h, Bind (Return v) c2) (h, c2 v)
+
+  | StepLoop : forall (acc : Set) (init : acc) (body : acc -> cmd (loop_outcome acc)) h,
+    step (h, Loop init body) (h, o <- body init; match o with
+                                                 | Done a => Return a
+                                                 | Again a => Loop a body
+                                                 end)
+
+  | StepRead : forall h a v,
+    h $? a = Some v
+    -> step (h, Read a) (h, Return v)
+  | StepWrite : forall h a v v',
+    h $? a = Some v
+    -> step (h, Write a v') (h $+ (a, v'), Return tt).
+
+
+  Definition trsys_of (h : heap) {result} (c : cmd result) := {|
+    Initial := {(h, c)};
+    Step := step (A := result)
+  |}.
+
+  Definition multistep_trsys_of (h : heap) {result} (c : cmd result) := {|
+    Initial := {(h, c)};
+    Step := (step (A := result))^*
+  |}.
+
+  (* Now let's get into the first distinctive feature of separation logic: an
+   * assertion language that takes advantage of *partiality* of heaps.  We give our
+   * definitions inside a module, which will shortly be used as a parameter to
+   * another module (from the book library), to get some free automation for
+   * implications between these assertions. *)
   Module Import S <: SEP.
     Definition hprop := heap -> Prop.
+    (* A [hprop] is a regular old assertion over heaps. *)
 
+    (* Implication *)
     Definition himp (p q : hprop) := forall h, p h -> q h.
+
+    (* Equivalence *)
     Definition heq (p q : hprop) := forall h, p h <-> q h.
 
+    (* Lifting a pure proposition: it must hold, and the heap must be empty. *)
     Definition lift (P : Prop) : hprop :=
       fun h => P /\ h = $0.
 
+    (* Separating conjunction, one of the two big ideas of separation logic.
+     * When does [star p q] apply to [h]?  When [h] can be partitioned into two
+     * subheaps [h1] and [h2], respectively compatible with [p] and [q].  See book
+     * module [Map] for definitions of [split] and [disjoint]. *)
     Definition star (p q : hprop) : hprop :=
       fun h => exists h1 h2, split h h1 h2 /\ disjoint h1 h2 /\ p h1 /\ q h2.
 
+    (* Existential quantification *)
     Definition exis {A} (p : A -> hprop) : hprop :=
       fun h => exists x, p x h.
 
+    (* Convenient notations *)
     Notation "[| P |]" := (lift P) : sep_scope.
     Infix "*" := star : sep_scope.
     Notation "'exists' x .. y , p" := (exis (fun x => .. (exis (fun y => p)) ..)) : sep_scope.
@@ -314,6 +257,9 @@ Module DeeplyEmbedded(Import BW : BIT_WIDTH).
     Notation "p ===> q" := (himp p%sep q%sep) (no associativity, at level 70).
 
     Local Open Scope sep_scope.
+
+    (* And now we prove some key algebraic properties, whose details aren't so
+     * important.  The library automation uses these properties. *)
 
     Lemma iff_two : forall A (P Q : A -> Prop),
       (forall x, P x <-> Q x)
@@ -326,7 +272,7 @@ Module DeeplyEmbedded(Import BW : BIT_WIDTH).
                     repeat (match goal with
                             | [ H : forall x, _ <-> _ |- _  ] =>
                               apply iff_two in H
-                            | [ H : ex _ |- _ ] => cases H
+                            | [ H : ex _ |- _ ] => destruct H
                             | [ H : split _ _ $0 |- _ ] => apply split_empty_fwd in H
                             end; propositional; subst); eauto 15.
 
@@ -410,13 +356,17 @@ Module DeeplyEmbedded(Import BW : BIT_WIDTH).
   End S.
 
   Export S.
+  (* Instantiate our big automation engine to these definitions. *)
   Module Import Se := SepCancel.Make(S).
+  Export Se.
 
-  Definition heap1 (a : wrd) (p : value * value) : heap := $0 $+ (a, p).
-  Definition ptsto (a : wrd) (p : value * value) : hprop :=
-    fun h => h = heap1 a p.
 
-  (* Helpful notations, some the same as above *)
+  (* ** Predicates *)
+
+  Definition heap1 (a v : wrd) : heap := $0 $+ (a, v).
+  Definition ptsto (a v : wrd) : hprop :=
+    fun h => h = heap1 a v.
+
   Notation "[| P |]" := (lift P) : sep_scope.
   Notation emp := (lift True).
   Infix "*" := star : sep_scope.
@@ -426,952 +376,1044 @@ Module DeeplyEmbedded(Import BW : BIT_WIDTH).
   Notation "p ===> q" := (himp p%sep q%sep) (no associativity, at level 70).
   Infix "|->" := ptsto (at level 30) : sep_scope.
 
+  Fixpoint multi_ptsto (a : wrd) (vs : list wrd) : hprop :=
+    match vs with
+    | nil => emp
+    | v :: vs' => a |-> v * multi_ptsto (a ^+ ^1) vs'
+    end%sep.
+
+  Infix "|-->" := multi_ptsto (at level 30) : sep_scope.
+
 
   (** * Finally, the Hoare logic *)
 
-  Definition hassert := valuation -> hprop.
+  Inductive hoare_triple : forall {result}, hprop -> cmd result -> (result -> hprop) -> Prop :=
+  | HtReturn : forall P {result : Set} (v : result),
+      hoare_triple P (Return v) (fun r => P * [| r = v |])%sep
+  | HtBind : forall P {result' result} (c1 : cmd result') (c2 : result' -> cmd result) Q R,
+      hoare_triple P c1 Q
+      -> (forall r, hoare_triple (Q r) (c2 r) R)
+      -> hoare_triple P (Bind c1 c2) R
+  | HtLoop : forall {acc : Set} (init : acc) (body : acc -> cmd (loop_outcome acc)) I,
+      (forall acc, hoare_triple (I (Again acc)) (body acc) I)
+      -> hoare_triple (I (Again init)) (Loop init body) (fun r => I (Done r))
+  | HtFail : forall {result},
+      hoare_triple (fun _ => False) (Fail (result := result)) (fun _ _ => False)
 
-  Inductive hoare_triple_exp : hassert -> exp -> (value -> hassert) -> Prop :=
-  | HtVar : forall x,
-      hoare_triple_exp (fun V => exists v, [| V $? x = Some v |])%sep
-                       (Var x)
-                       (fun r V => [| V $? x = Some r |])%sep
-  | HtConst : forall n,
-      hoare_triple_exp (fun _ => emp)%sep
-                       (Const n)
-                       (fun r _ => [| r = VScalar n |])%sep
-  | HtAdd : forall x n,
-      hoare_triple_exp (fun V => exists xn, [| V $? x = Some (VScalar xn) |])%sep
-                       (Add x n)
-                       (fun r V => exists xn, [| V $? x = Some (VScalar xn) |]
-                                              * [| r = VScalar (xn ^+ n) |])%sep
-  | HtHead : forall R x,
-      hoare_triple_exp (fun V => exists a, [| V $? x = Some (VList a) |]
-                                           * exists p, a |-> p * R p)%sep
-                       (Head x)
-                       (fun r V => exists a, [| V $? x = Some (VList a) |]
-                                             * exists vt, a |-> (r, vt) * R (r, vt))%sep
-  | HtTail : forall R x,
-      hoare_triple_exp (fun V => exists a, [| V $? x = Some (VList a) |]
-                                           * exists p, a |-> p * R p)%sep
-                       (Tail x)
-                       (fun r V => exists a, [| V $? x = Some (VList a) |]
-                                             * exists vh, a |-> (vh, r) * R (vh, r))%sep
-  | HtNotNull : forall x,
-      hoare_triple_exp (fun V => exists a, [| V $? x = Some (VList a) |])%sep
-                       (NotNull x)
-                       (fun r V => exists a, [| V $? x = Some (VList a) |]
-                                             * [| r = VScalar (if weq a (^0) then ^1 else ^0) |])%sep
-  | HtExpConsequence : forall P e Q P' Q',
-      hoare_triple_exp P e Q
-      -> (forall V, P' V ===> P V)
-      -> (forall r V, Q r V ===> Q' r V)
-      -> hoare_triple_exp P' e Q'
-  | HtExpFrame : forall P e Q R,
-      hoare_triple_exp P e Q
-      -> hoare_triple_exp (fun V => P V * R V)%sep e (fun r V => Q r V * R V)%sep.
+  | HtRead : forall a R,
+      hoare_triple (exists v, a |-> v * R v)%sep (Read a) (fun r => a |-> r * R r)%sep
+  | HtWrite : forall a v',
+      hoare_triple (exists v, a |-> v)%sep (Write a v') (fun _ => a |-> v')%sep
 
-  Fixpoint couldChange (s : stmt) (x : var) : bool :=
-    match s with
-    | Skip => false
-    | Assign y _ => if y ==v x then true else false
-    | WriteHead _ _
-    | WriteTail _ _ => false
-    | Seq s1 s2 => couldChange s1 x || couldChange s2 x
-    | IfThenElse _ s1 s2 => couldChange s1 x || couldChange s2 x
-    | WhileLoop _ s1 => couldChange s1 x
-    end.
+  | HtConsequence : forall {result} (c : cmd result) P Q (P' : hprop) (Q' : _ -> hprop),
+      hoare_triple P c Q
+      -> P' ===> P
+      -> (forall r, Q r ===> Q' r)
+      -> hoare_triple P' c Q'
 
-  Inductive hoare_triple : hassert -> stmt -> hassert -> Prop :=
-  | HtSkip : forall P,
-      hoare_triple P Skip P
-  | HtAssign : forall P x e Q,
-      hoare_triple_exp P e Q
-      -> hoare_triple P (Assign x e) (fun V => exists V' r, Q r V' * [| V = V' $+ (x, r) |])%sep
-  | HtWriteHead : forall P x e R,
-      hoare_triple_exp P e (fun r V => exists a, [| V $? x = Some (VList a) |] * exists vhd vtl, a |-> (vhd, vtl) * R r vhd vtl V)%sep
-      -> hoare_triple P
-                      (WriteHead x e)
-                      (fun V => exists a, [| V $? x = Some (VList a) |] * exists r vhd vtl, a |-> (r, vtl) * R r vhd vtl V)%sep
-  | HtWriteTail : forall P x e R,
-      hoare_triple_exp P e (fun r V => exists a, [| V $? x = Some (VList a) |] * exists vhd vtl, a |-> (vhd, vtl) * R r vhd vtl V)%sep
-      -> hoare_triple P
-                      (WriteTail x e)
-                      (fun V => exists a, [| V $? x = Some (VList a) |] * exists r vhd vtl, a |-> (vhd, r) * R r vhd vtl V)%sep
-  | HtSeq : forall P s1 Q s2 R,
-      hoare_triple P s1 Q
-      -> hoare_triple Q s2 R
-      -> hoare_triple P (Seq s1 s2) R
-  | HtIfThenElse : forall P e s1 s2 Q R,
-      hoare_triple_exp P e (fun r V => Q r V * exists n, [| r = VScalar n |])%sep
-      -> hoare_triple (fun V => exists n, Q (VScalar n) V * [| n <> ^0 |])%sep s1 R
-      -> hoare_triple (fun V => Q (VScalar (^0)) V)%sep s2 R
-      -> hoare_triple P (IfThenElse e s1 s2) R
-  | HtWhileLoop : forall I e s1 Q,
-      hoare_triple_exp I e (fun r V => Q r V * exists n, [| r = VScalar n |])%sep
-      -> hoare_triple (fun V => exists n, Q (VScalar n) V * [| n <> ^0 |])%sep s1 I
-      -> hoare_triple I (WhileLoop e s1) (Q (VScalar (^0)))
-  | HtConsequence : forall P s Q P' Q',
-      hoare_triple P s Q
-      -> (forall V, P' V ===> P V)
-      -> (forall V, Q V ===> Q' V)
-      -> hoare_triple P' s Q'
-  | HtFrame : forall P s Q R,
-      hoare_triple P s Q
-      -> (forall V1 V2, (forall x, couldChange s x = false
-                                   -> V1 $? x = V2 $? x)
-                        -> R V1 = R V2)
-      -> hoare_triple (fun V => P V * R V)%sep s (fun V => Q V * R V)%sep.
+  | HtFrame : forall {result} (c : cmd result) P Q R,
+      hoare_triple P c Q
+      -> hoare_triple (P * R)%sep c (fun r => Q r * R)%sep.
 
-  Notation "{{ V1 ~> P }} c {{ V2 ~> Q }}" :=
-    (hoare_triple (fun V1 => P%sep) c (fun V2 => Q%sep)) (at level 90, c at next level).
 
-  Lemma HtStrengthen : forall P s Q Q',
-      hoare_triple P s Q
-      -> (forall V, Q V ===> Q' V)
-      -> hoare_triple P s Q'.
+  Notation "{{ P }} c {{ r ~> Q }}" :=
+    (hoare_triple P%sep c (fun r => Q%sep)) (at level 90, c at next level).
+
+  Lemma HtStrengthen : forall {result} (c : cmd result) P Q (Q' : _ -> hprop),
+      hoare_triple P c Q
+      -> (forall r, Q r ===> Q' r)
+      -> hoare_triple P c Q'.
   Proof.
     simplify.
     eapply HtConsequence; eauto.
     reflexivity.
   Qed.
 
-  Lemma HtWeaken : forall P s Q P',
-      hoare_triple P s Q
-      -> (forall V, P' V ===> P V)
-      -> hoare_triple P' s Q.
+  Lemma HtWeaken : forall {result} (c : cmd result) P Q (P' : hprop),
+      hoare_triple P c Q
+      -> P' ===> P
+      -> hoare_triple P' c Q.
   Proof.
     simplify.
     eapply HtConsequence; eauto.
     reflexivity.
   Qed.
 
-  Definition trsys_of (H : heap) (V : valuation) (s : stmt) := {|
-    Initial := constant [(H, V, s)];
-    Step := step
-  |}.
+  (* Now, we carry out a moderately laborious soundness proof!  It's safe to skip
+   * ahead to the text "Examples", but a few representative lemma highlights
+   * include [invert_Read], [preservation], [progress], and the main theorem
+   * [hoare_triple_sound]. *)
 
-  Hint Constructors hoare_triple_exp hoare_triple eval step.
-
-  Lemma eval_subheap : forall H V e r,
-      eval H V e r
-      -> forall H', (forall a v, H $? a = Some v -> H' $? a = Some v)
-                    -> eval H' V e r.
-  Proof.
-    invert 1; simplify; eauto.
-  Qed.
-
-  Lemma drop_cells : forall P e Q,
-      hoare_triple_exp P e Q
-      -> forall V H r, eval H V e r
-                       -> forall H', P V H'
-                                     -> (forall a v, H' $? a = Some v -> H $? a = Some v)
-                                     -> eval H' V e r.
-  Proof.
-    induct 1; simplify.
-
-    invert H0; auto.
-
-    invert H0; auto.
-
-    invert H0; auto.
-
-    invert H0.
-    invert H1.
-    invert H0; simp.
-    invert H3.
-    apply split_empty_fwd' in H1; subst.
-    invert H6.
-    invert H1; simp.
-    econstructor.
-    eassumption.
-    cases (x2 $? x0).
-    apply H2 in Heq.
-    replace p0 with (r, pt) by equality.
-    eauto.
-    unfold split in H3; subst.
-    unfold ptsto in H6; subst.
-    unfold heap1 in Heq.
-    rewrite lookup_join1 in Heq by (simplify; sets).
-    simplify; equality.
-
-    invert H0.
-    invert H1.
-    invert H0; simp.
-    invert H3.
-    apply split_empty_fwd' in H1; subst.
-    invert H6.
-    invert H1; simp.
-    econstructor.
-    eassumption.
-    cases (x2 $? x0).
-    apply H2 in Heq.
-    replace p0 with (ph, r) by equality.
-    eauto.
-    unfold split in H3; subst.
-    unfold ptsto in H6; subst.
-    unfold heap1 in Heq.
-    rewrite lookup_join1 in Heq by (simplify; sets).
-    simplify; equality.
-
-    invert H0; auto.
-
-    eapply IHhoare_triple_exp; eauto.
-    apply H0; auto.
-
-    invert H2; simp.
-    eapply IHhoare_triple_exp in H1.
-    2: eauto.
-    eapply eval_subheap; eauto.
-    simplify.
-    unfold split in H4; subst.
-    rewrite lookup_join1 by eauto using lookup_Some_dom.
-    auto.
-    simplify.
-    unfold split in H4; subst.
-    apply H3.
-    rewrite lookup_join1 by eauto using lookup_Some_dom.
-    auto.
-  Qed.
-
-  Lemma preservation_exp : forall P e Q,
-      hoare_triple_exp P e Q
-      -> forall V H r, P V H -> eval H V e r -> Q r V H.
-  Proof.
-    induct 1; simplify.
-
-    invert H1.
-    cases H0.
-    cases H0.
-    constructor; assumption.
-
-    invert H1.
-    invert H0.
-    constructor; reflexivity.
-
-    invert H1.
-    invert H0.
-    invert H1.
-    eexists.
-    exists $0, $0; propositional; eauto.
-    constructor; eauto.
-    constructor; equality.
-
-    invert H1.
-    invert H0.
-    invert H1.
-    simp.
-    invert H2.
-    invert H5.
-    cases x1.
-    replace r with v.
-    exists x0.
-    exists $0, H; propositional; eauto.
-    constructor; auto.
-    exists v0.
-    apply split_empty_fwd' in H0; equality.
-    invert H2; simp.
-    unfold split in H5; subst.
-    unfold ptsto in H6; subst.
-    apply split_empty_fwd' in H0; subst.
-    replace x0 with p in * by equality.
-    unfold heap1 in H7.
-    simplify.
-    rewrite lookup_join1 in H7.
-    simplify; equality.
-    simplify; sets.
-
-    invert H1.
-    invert H0.
-    invert H1.
-    simp.
-    invert H2.
-    invert H5.
-    cases x1.
-    replace r with v0.
-    exists x0.
-    exists $0, H; propositional; eauto.
-    constructor; auto.
-    exists v.
-    apply split_empty_fwd' in H0; equality.
-    invert H2; simp.
-    unfold split in H5; subst.
-    unfold ptsto in H6; subst.
-    apply split_empty_fwd' in H0; subst.
-    replace x0 with p in * by equality.
-    unfold heap1 in H7.
-    simplify.
-    rewrite lookup_join1 in H7.
-    simplify; equality.
-    simplify; sets.
-
-    invert H1.
-    invert H0.
-    invert H1.
-    exists p, $0, $0; propositional; eauto.
-    constructor; auto.
-    constructor; auto.
-
-    unfold himp in *; eauto.
-
-    invert H1; simp.
-    exists x, x0; propositional; eauto.
-    eapply IHhoare_triple_exp; eauto.
-    eapply drop_cells; eauto.
-    simplify.
-    unfold split in H3; subst.
-    rewrite lookup_join1 by eauto using lookup_Some_dom.
-    auto.
-  Qed.
-
-  Opaque heq himp lift star exis ptsto.
-
-  Lemma invert_Assign : forall P x e Q,
-    hoare_triple P (Assign x e) Q
-    -> exists Q', hoare_triple_exp P e Q'
-                  /\ forall V r, Q' r V ===> Q (V $+ (x, r)).
+  Lemma invert_Return : forall {result : Set} (r : result) P Q,
+    hoare_triple P (Return r) Q
+    -> forall h, P h -> Q r h.
   Proof.
     induct 1; propositional; eauto.
 
-    do 2 eexists.
-    eassumption.
-    simplify.
-    do 2 eapply exis_right.
-    cancel.
+    exists h, $0; propositional; eauto.
+    unfold lift; propositional.
 
-    first_order.
-    do 2 eexists.
-    eapply HtExpConsequence.
-    eassumption.
-    assumption.
-    reflexivity.
-    etransitivity; eauto.
+    unfold himp in *; eauto.
 
-    first_order.
-    do 2 eexists.
-    eapply HtExpFrame.
-    eassumption.
-    simplify.
-    rewrite H0 with (V1 := V) (V2 := V $+ (x, r)).
-    rewrite H2.
-    reflexivity.
-    simplify.
-    cases (x ==v x1); simplify; equality.
+    unfold star, himp in *; simp; eauto 7.
   Qed.
 
-  Lemma invert_WriteHead : forall P x e Q,
-    hoare_triple P (WriteHead x e) Q
-    -> exists R, hoare_triple_exp P e (fun r V => exists a, [| V $? x = Some (VList a) |] * exists vhd vtl, a |-> (vhd, vtl) * R r vhd vtl V)%sep
-                  /\ (forall V, (exists a, [| V $? x = Some (VList a) |] * exists r vhd vtl, a |-> (r, vtl) * R r vhd vtl V) ===> Q V).
+  Hint Constructors hoare_triple.
+
+  Lemma invert_Bind : forall {result' result} (c1 : cmd result') (c2 : result' -> cmd result) P Q,
+    hoare_triple P (Bind c1 c2) Q
+    -> exists R, hoare_triple P c1 R
+                 /\ forall r, hoare_triple (R r) (c2 r) Q.
   Proof.
-    induct 1; first_order; eauto.
+    induct 1; propositional; eauto.
 
-    do 2 eexists.
-    eassumption.
-    reflexivity.
-
-    do 2 eexists.
-    eapply HtExpConsequence.
-    eassumption.
-    assumption.
-    simplify.
-    reflexivity.
-    etransitivity; eauto.
-
-    exists (fun r vhd vtl V => x0 r vhd vtl V * R V)%sep.
-    propositional.
-    eapply HtExpConsequence with (Q := fun r V =>
-                                         ((exists a, [|V $? x = Some (VList a)|]
-                                                    * exists vhd vtl, a |-> (vhd, vtl) * x0 r vhd vtl V) * R V)%sep).
-    eapply HtExpFrame.
-    eassumption.
-    reflexivity.
-    cancel.
-    rewrite <- H2.
-    cancel.
-  Qed.
-
-  Lemma invert_WriteTail : forall P x e Q,
-    hoare_triple P (WriteTail x e) Q
-    -> exists R, hoare_triple_exp P e (fun r V => exists a, [| V $? x = Some (VList a) |] * exists vhd vtl, a |-> (vhd, vtl) * R r vhd vtl V)%sep
-                  /\ (forall V, (exists a, [| V $? x = Some (VList a) |] * exists r vhd vtl, a |-> (vhd, r) * R r vhd vtl V) ===> Q V).
-  Proof.
-    induct 1; first_order; eauto.
-
-    do 2 eexists.
-    eassumption.
-    reflexivity.
-
-    do 2 eexists.
-    eapply HtExpConsequence.
-    eassumption.
-    assumption.
-    simplify.
-    reflexivity.
-    etransitivity; eauto.
-
-    exists (fun r vhd vtl V => x0 r vhd vtl V * R V)%sep.
-    propositional.
-    eapply HtExpConsequence with (Q := fun r V =>
-                                         ((exists a, [|V $? x = Some (VList a)|]
-                                                    * exists vhd vtl, a |-> (vhd, vtl) * x0 r vhd vtl V) * R V)%sep).
-    eapply HtExpFrame.
-    eassumption.
-    reflexivity.
-    cancel.
-    rewrite <- H2.
-    cancel.
-  Qed.
-
-  Lemma invert_Skip : forall P Q,
-    hoare_triple P Skip Q
-    -> forall V, P V ===> Q V.
-  Proof.
-    induct 1; simplify.
-
-    reflexivity.
-
-    do 2 (etransitivity; eauto).
-
-    rewrite IHhoare_triple.
-    reflexivity.
-  Qed.
-
-  Lemma invert_Seq : forall P s1 s2 Q,
-    hoare_triple P (Seq s1 s2) Q
-    -> exists R, hoare_triple P s1 R
-                 /\ hoare_triple R s2 Q.
-  Proof.
-    induct 1; simplify; first_order.
-
-    do 2 eexists.
-    eapply HtConsequence; eauto; reflexivity.
-    eapply HtConsequence; eauto; reflexivity.
-
-    do 2 eexists.
-    eapply HtFrame; eauto.
-    simplify.
-    apply H0.
-    simplify.
-    apply orb_false_elim in H4; propositional; eauto.
-    eapply HtFrame; eauto.
-    simplify.
-    apply H0.
-    simplify.
-    apply orb_false_elim in H4; propositional; eauto.
-  Qed.
-
-  Lemma invert_IfThenElse : forall P e s1 s2 Q,
-    hoare_triple P (IfThenElse e s1 s2) Q
-    -> exists R, hoare_triple_exp P e (fun r V => R r V * exists n, [| r = VScalar n |])%sep
-                 /\ hoare_triple (fun V => exists n, R (VScalar n) V * [| n <> ^0 |])%sep s1 Q
-                 /\ hoare_triple (fun V => R (VScalar (^0)) V)%sep s2 Q.
-  Proof.
-    induct 1; simplify; first_order.
-
+    invert IHhoare_triple; propositional.
     eexists; propositional.
-    eapply HtExpConsequence.
-    eassumption.
-    assumption.
-    simplify.
-    reflexivity.
-    eapply HtStrengthen.
-    eassumption.
-    assumption.
-    eapply HtStrengthen.
-    eassumption.
-    assumption.
-
-    exists (fun r V => x r V * R V)%sep; propositional.
-    eapply HtExpConsequence.
-    eapply HtExpFrame.
-    eauto.
-    simplify.
-    reflexivity.
-    simplify.
-    cancel.
-    eauto.
     eapply HtWeaken.
-    eapply HtFrame.
     eassumption.
-    simplify.
-    apply H0.
-    simplify.
-    apply orb_false_elim in H5; propositional; eauto.
-    simplify.
-    cancel.
-    eapply HtFrame.
-    assumption.
-    simplify.
-    apply H0.
-    simplify.
-    apply orb_false_elim in H5; propositional; eauto.
+    auto.
+    eapply HtStrengthen.
+    apply H4.
+    auto.
+
+    simp.
+    exists (fun r => x r * R)%sep.
+    propositional.
+    eapply HtFrame; eauto.
+    eapply HtFrame; eauto.
   Qed.
 
-  Lemma invert_WhileLoop : forall P e s1 Q,
-    hoare_triple P (WhileLoop e s1) Q
-    -> exists I R, (forall V, P V ===> I V)
-                   /\ hoare_triple_exp I e (fun r V => R r V * exists n, [| r = VScalar n |])%sep
-                   /\ hoare_triple (fun V => exists n, R (VScalar n) V * [| n <> ^0 |])%sep s1 I
-                   /\ (forall V, R (VScalar (^0)) V ===> Q V).
+  Lemma invert_Loop : forall {acc : Set} (init : acc) (body : acc -> cmd (loop_outcome acc)) P Q,
+      hoare_triple P (Loop init body) Q
+      -> exists I, (forall acc, hoare_triple (I (Again acc)) (body acc) I)
+                   /\ (forall h, P h -> I (Again init) h)
+                   /\ (forall r h, I (Done r) h -> Q r h).
   Proof.
-    induct 1; simplify; first_order.
+    induct 1; propositional; eauto.
 
-    do 2 eexists; propositional; eauto; reflexivity.
+    invert IHhoare_triple; propositional.
+    exists x; propositional; eauto.
+    unfold himp in *; eauto.
 
-    exists x, x0; propositional.
-    etransitivity; eauto.
-    etransitivity; eauto.
-
-    exists (fun V => x V * R V)%sep, (fun r V => x0 r V * R V)%sep; propositional.
-    rewrite H1; reflexivity.
-    eapply HtExpConsequence.
-    eapply HtExpFrame.
-    eauto.
-    simplify.
-    reflexivity.
-    simplify.
-    cancel.
-    eauto.
-    eapply HtWeaken.
-    eauto.
-    simplify.
-    cancel.
-    rewrite H4.
-    reflexivity.
+    simp.
+    exists (fun o => x o * R)%sep; propositional; eauto.
+    unfold star in *; simp; eauto 7.
+    unfold star in *; simp; eauto 7.
   Qed.
 
+  Lemma invert_Fail : forall result P Q,
+    hoare_triple P (Fail (result := result)) Q
+    -> forall h, P h -> False.
+  Proof.
+    induct 1; propositional; eauto.
+
+    unfold star in *; simp; eauto.
+  Qed.
+
+  (* Now that we proved enough basic facts, let's hide the definitions of all
+   * these predicates, so that we reason about them only through automation. *)
+  Opaque heq himp lift star exis ptsto.
+
+  Lemma unit_not_wrd : unit = wrd -> False.
+  Proof.
+    simplify.
+    assert (exists x : unit, forall y : unit, x = y).
+    exists tt; simplify.
+    cases y; reflexivity.
+    rewrite H in H0.
+    invert H0.
+    specialize (H1 (x ^+ ^1)).
+    eapply adding_one_changes.
+    apply bit_width_nonzero.
+    symmetry; eassumption.
+  Qed.
+
+  Lemma invert_Read : forall a P Q,
+    hoare_triple P (Read a) Q
+    -> exists R, (P ===> exists v, a |-> v * R v)%sep
+                 /\ forall r, a |-> r * R r ===> Q r.
+  Proof.
+    induct 1; simp; eauto.
+
+    exists R; simp.
+    cancel; auto.
+    cancel; auto.
+
+    apply unit_not_wrd in x0; simp.
+
+    specialize (IHhoare_triple _ _ eq_refl JMeq.JMeq_refl JMeq.JMeq_refl); first_order.
+    exists x.
+    propositional.
+    etransitivity; eauto.
+    etransitivity; eauto.
+
+    specialize (IHhoare_triple _ _ eq_refl JMeq.JMeq_refl JMeq.JMeq_refl); first_order.
+    exists (fun n => x n * R)%sep; simp.
+    rewrite H0.
+    cancel.
+
+    rewrite <- H1.
+    cancel.
+  Qed.
+
+  Lemma invert_Write : forall a v' P Q,
+    hoare_triple P (Write a v') Q
+    -> exists R, (P ===> (exists v, a |-> v) * R)%sep
+                 /\ a |-> v' * R ===> Q tt.
+  Proof.
+    induct 1; simp; eauto.
+
+    symmetry in x0.
+    apply unit_not_wrd in x0; simp.
+
+    exists emp; simp.
+    cancel; auto.
+    cancel; auto.
+
+    eexists; split.
+    etransitivity; eauto.
+    etransitivity; eauto.
+
+    exists (x * R)%sep; simp.
+    rewrite H1.
+    cancel.
+
+    cancel.
+    rewrite <- H2.
+    cancel.
+  Qed.
+
+  Lemma HtReturn' : forall P {result : Set} (v : result) Q,
+      P ===> Q v
+      -> hoare_triple P (Return v) Q.
+  Proof.
+    simp.
+    eapply HtStrengthen.
+    constructor.
+    simp.
+    cancel.
+  Qed.
+
+  (* Temporarily transparent again! *)
   Transparent heq himp lift star exis ptsto.
 
-  Lemma preservation : forall s H V s' V' H',
-      step (H, V, s) (H', V', s')
-      -> forall Q, hoare_triple (fun V' H' => H' = H /\ V' = V) s Q
-                   -> hoare_triple (fun V'' H'' => H'' = H' /\ V'' = V') s' Q.
+  Lemma preservation : forall {result} (c : cmd result) h c' h',
+      step (h, c) (h', c')
+      -> forall Q, hoare_triple (fun h' => h' = h) c Q
+                   -> hoare_triple (fun h'' => h'' = h') c' Q.
   Proof.
     induct 1; simplify.
 
-    apply invert_Assign in H; simp.
-    eapply preservation_exp in H0; eauto.
-    eapply HtWeaken.
-    auto.
-    unfold himp; simplify.
-    propositional; subst.
-    apply H2; assumption.
-    simplify; auto.
-
-    apply invert_WriteHead in H3; simp.
-    eapply preservation_exp in H1; eauto.
-    simplify.
-    eapply HtWeaken.
-    auto.
-    unfold himp; simplify.
-    propositional; subst.
-    apply H5.
-    invert H1.
-    invert H4; simp.
-    invert H6.
-    invert H8.
-    invert H6.
-    invert H8; simp.
-    invert H9.
-    exists x1.
-    apply split_empty_fwd' in H1; subst.
-    exists $0, (x3 $+ (a, (v, tv))); propositional; eauto.
-    constructor; auto.
-    exists v, x2, tv.
-    exists (heap1 x1 (v, tv)), x6; propositional; eauto.
-    unfold split, heap1.
-    unfold split, heap1 in H6.
-    subst.
-    apply fmap_ext; simplify.
-    cases (weq k x1); subst.
-    replace x1 with a by equality.
-    repeat (rewrite lookup_join1 by (simplify; sets); simplify).
-    auto.
-    simplify.
-    repeat (rewrite lookup_join2 by (simplify; sets); simplify).
-    auto.
-    unfold disjoint, heap1 in *.
-    intros.
-    apply H8 with a0.
-    cases (weq x1 a0); subst; simplify.
-    equality.
-    assumption.
-    assumption.
-    constructor.
-    unfold split in H6; subst.
-    replace x1 with a in * by equality.
-    unfold heap1 in H2.
-    rewrite lookup_join1 in H2 by (simplify; sets).
-    simplify.
-    equality.
-    simplify; auto.
-
-    apply invert_WriteTail in H3; simp.
-    eapply preservation_exp in H1; eauto.
-    simplify.
-    eapply HtWeaken.
-    auto.
-    unfold himp; simplify.
-    propositional; subst.
-    apply H5.
-    invert H1.
-    invert H4; simp.
-    invert H6.
-    invert H8.
-    invert H6.
-    invert H8; simp.
-    invert H9.
-    exists x1.
-    apply split_empty_fwd' in H1; subst.
-    exists $0, (x3 $+ (a, (hv, v))); propositional; eauto.
-    constructor; auto.
-    exists v, hv, x4.
-    exists (heap1 x1 (hv, v)), x6; propositional; eauto.
-    unfold split, heap1.
-    unfold split, heap1 in H6.
-    subst.
-    apply fmap_ext; simplify.
-    cases (weq k x1); subst.
-    replace x1 with a by equality.
-    repeat (rewrite lookup_join1 by (simplify; sets); simplify).
-    auto.
-    simplify.
-    repeat (rewrite lookup_join2 by (simplify; sets); simplify).
-    auto.
-    unfold disjoint, heap1 in *.
-    intros.
-    apply H8 with a0.
-    cases (weq x1 a0); subst; simplify.
-    equality.
-    assumption.
-    assumption.
-    constructor.
-    unfold split in H6; subst.
-    replace x1 with a in * by equality.
-    unfold heap1 in H2.
-    rewrite lookup_join1 in H2 by (simplify; sets).
-    simplify.
-    equality.
-    simplify; auto.
-
-    apply invert_Seq in H; first_order.
-    eapply HtWeaken.
-    eauto.
-    simplify.
-    eapply invert_Skip in H; eassumption.
-
-    apply invert_Seq in H1; first_order.
+    apply invert_Bind in H0; simp.
     eauto.
 
-    apply invert_IfThenElse in H; first_order.
-    eapply HtWeaken; eauto.
-    simplify.
-    unfold himp; propositional; subst.
-    eapply preservation_exp in H0; eauto.
-    exists n, H', $0; propositional; eauto.
-    invert H0; simp.
-    invert H7.
-    invert H6.
-    apply split_empty_fwd in H4; subst.
-    auto.
-    constructor; auto.
-    simplify; auto.
+    apply invert_Bind in H; simp.
+    specialize (invert_Return _ _ _ H); eauto using HtWeaken.
 
-    apply invert_IfThenElse in H; first_order.
-    eapply HtWeaken; eauto.
-    simplify.
-    unfold himp; propositional; subst.
-    eapply preservation_exp in H0; eauto.
-    eapply HtExpConsequence.
+    apply invert_Loop in H; simp.
+    econstructor.
+    eapply HtWeaken.
     eauto.
-    simplify.
-    instantiate (1 := fun V H'0 => H'0 = H' /\ V = V').
-    simplify.
-    reflexivity.
-    simplify.
-    unfold himp; simplify.
-    invert H3; simp.
-    invert H7.
-    invert H6.
-    apply split_empty_fwd in H4; subst.
-    auto.
-    simplify; auto.
-
-    apply invert_WhileLoop in H; first_order.
-    eapply HtSeq.
-    eapply HtWeaken; eauto.
-    simplify.
-    unfold himp; propositional; subst.
-    eapply preservation_exp in H0; eauto.
-    exists n, H', $0; propositional; eauto.
-    invert H0; simp.
-    invert H8.
-    invert H7.
-    apply split_empty_fwd in H5; subst.
-    auto.
-    constructor; auto.
-    apply H; simplify; auto.
+    assumption.
+    simp.
+    cases r.
+    apply HtReturn'.
+    unfold himp; simp; eauto.
     eapply HtStrengthen.
     eauto.
-    eauto.
+    unfold himp; simp; eauto.
 
-    apply invert_WhileLoop in H; first_order.
-    eapply HtWeaken; eauto.
-    simplify.
-    unfold himp; propositional; subst.
-    eapply preservation_exp in H0; eauto.
-    apply H3; auto.
-    simplify.
-    invert H0; simp.
-    invert H7.
-    invert H6.
-    apply split_empty_fwd in H4; subst.
-    auto.
-    apply H; simplify; auto.
+    apply invert_Read in H0; simp.
+    apply HtReturn'.
+    assert ((exists v, a |-> v * x v)%sep h') by auto.
+    unfold exis, star in H1; simp.
+    unfold ptsto in H4; subst.
+    unfold split in H1; subst.
+    unfold heap1 in H.
+    rewrite lookup_join1 in H by (simp; sets).
+    unfold himp; simp.
+    invert H.
+    apply H2.
+    unfold star.
+    exists (heap1 a v), x2; propositional.
+    unfold split; reflexivity.
+    unfold ptsto; reflexivity.
+
+    apply invert_Write in H0; simp.
+    apply HtReturn'.
+    simp.
+    assert (((exists v : wrd, a |-> v) * x)%sep h) by auto.
+    unfold star in H1; simp.
+    invert H4.
+    unfold ptsto in H5; subst.
+    unfold split in H3; subst.
+    unfold heap1 in H.
+    rewrite lookup_join1 in H by (simp; sets).
+    unfold himp; simp.
+    invert H.
+    apply H2.
+    unfold star.
+    exists ($0 $+ (a, v')), x1; propositional.
+    unfold split.
+    unfold heap1.
+    maps_equal.
+    rewrite lookup_join1 by (simp; sets).
+    simp.
+    repeat rewrite lookup_join2 by (simp; sets); reflexivity.
+    unfold disjoint in *; simp.
+    cases (weq a0 a); simp.
+    apply H1 with (a0 := a).
+    unfold heap1; simp.
+    equality.
+    assumption.
+    unfold ptsto; reflexivity.
   Qed.
 
-  Lemma hoare_triple_sound' : forall P s Q,
-      hoare_triple P s Q
-      -> forall H V, P V H
-      -> invariantFor (trsys_of H V s)
-                      (fun p => hoare_triple (fun V' H' => H' = fst (fst p) /\ V' = snd (fst p))
-                                             (snd p)
-                                             Q).
+  Hint Constructors step.
+
+  Lemma progress : forall {result} (c : cmd result) P Q,
+      hoare_triple P c Q
+      -> forall h h1 h2, split h h1 h2
+                         -> disjoint h1 h2
+                         -> P h1
+                         -> (exists r, c = Return r)
+                            \/ (exists h' c', step (h, c) (h', c')).
+  Proof.
+    induct 1; simp;
+    repeat match goal with
+             | [ H : forall _ h1 _, _ -> _ -> ?P h1 -> _, H' : ?P _ |- _ ] => eapply H in H'; clear H; try eassumption; simp
+           end; eauto.
+
+    invert H1.
+    right; exists h, (Return x).
+    constructor.
+    unfold split, ptsto, heap1 in *; simp.
+    unfold star in H2; simp.
+    unfold split in H; simp.
+    rewrite lookup_join1; simp.
+    rewrite lookup_join1; simp.
+    sets.
+    eapply lookup_Some_dom.
+    rewrite lookup_join1; simp.
+    sets.
+
+    right; exists (h $+ (a, v')), (Return tt).
+    unfold split, exis, ptsto, heap1 in *; simp.
+    econstructor.
+    rewrite lookup_join1; simp.
+    sets.
+
+    unfold star in H2; simp.
+    apply IHhoare_triple with (h := h) (h1 := x) (h2 := h2 $++ x0); eauto.
+    unfold split in *; simp.
+    rewrite (@join_comm _ _ h2 x0).
+    apply join_assoc.
+    sets.
+    cases (h2 $? x1).
+    cases (x0 $? x1).
+    specialize (H2 x1).
+    specialize (H1 x1).
+    rewrite lookup_join2 in H1.
+    apply H1; equality.
+    unfold not.
+    simplify.
+    cases (x $? x1).
+    exfalso; apply H2; equality.
+    apply lookup_None_dom in Heq1; propositional.
+    apply lookup_None_dom in Heq0; propositional.
+    apply lookup_None_dom in Heq; propositional.
+
+    unfold split, disjoint in *; simp.
+    cases (h2 $? a).
+    rewrite lookup_join1 in H7.
+    apply H1 with (a := a); auto.
+    rewrite lookup_join1; auto.
+    cases (x $? a); try equality.
+    eauto using lookup_Some_dom.
+    eauto using lookup_Some_dom.
+    rewrite lookup_join2 in H7.
+    eapply H2; eassumption.
+    eauto using lookup_None_dom.
+  Qed.
+
+  Lemma hoare_triple_sound' : forall P {result} (c : cmd result) Q,
+      hoare_triple P c Q
+      -> P $0
+      -> invariantFor (trsys_of $0 c)
+                      (fun p =>
+                         hoare_triple (fun h' => h' = fst p)
+                                      (snd p)
+                                      Q).
   Proof.
     simplify.
 
     apply invariant_induction; simplify.
 
     propositional; subst; simplify.
-    eapply HtWeaken.
-    eauto.
+    eapply HtWeaken; eauto.
     unfold himp; simplify; equality.
 
-    cases s0.
-    cases p.
+    cases s.
     cases s'.
-    cases p.
-    simplify.
-    eapply preservation; eauto.
-  Qed.
-
-  Lemma progress_exp : forall P e Q,
-      hoare_triple_exp P e Q
-      -> forall V H H1 H2, split H H1 H2
-                           -> disjoint H1 H2
-                           -> P V H1
-                           -> exists v, eval H V e v.
-  Proof.
-    induct 1; simplify; eauto.
-
-    invert H4.
-    invert H5.
-    eauto.
-
-    invert H4.
-    invert H5.
-    eexists.
-    econstructor.
-    eauto.
-
-    invert H4.
-    invert H5; simp.
-    invert H6.
-    apply split_empty_fwd' in H4; subst.
-    invert H8.
-    invert H1; simp.
-    invert H6.
-    cases x1.
-    eexists.
-    econstructor.
-    eauto.
-    unfold heap1, split in *; subst.
-    rewrite lookup_join1.
-    rewrite lookup_join1.
-    simplify.
-    eauto.
-    eapply lookup_Some_dom; simplify; sets.
-    eapply lookup_Some_dom; simplify.
-    rewrite lookup_join1.
-    simplify; eauto.
-    eapply lookup_Some_dom; simplify; sets.
-
-    invert H4.
-    invert H5; simp.
-    invert H6.
-    apply split_empty_fwd' in H4; subst.
-    invert H8.
-    invert H1; simp.
-    invert H6.
-    cases x1.
-    eexists.
-    econstructor.
-    eauto.
-    unfold heap1, split in *; subst.
-    rewrite lookup_join1.
-    rewrite lookup_join1.
-    simplify.
-    eauto.
-    eapply lookup_Some_dom; simplify; sets.
-    eapply lookup_Some_dom; simplify.
-    rewrite lookup_join1.
-    simplify; eauto.
-    eapply lookup_Some_dom; simplify; sets.
-
-    invert H4.
-    invert H5.
-    eauto.
-
-    eapply IHhoare_triple_exp; eauto.
-    apply H0; auto.
-
-    invert H5; simp.
-    eapply IHhoare_triple_exp in H7; eauto.
-  Qed.
-
-  Lemma progress : forall P s Q,
-      hoare_triple P s Q
-      -> forall V H H1 H2, split H H1 H2
-                           -> disjoint H1 H2
-                           -> P V H1
-                           -> s = Skip \/ (exists H' V' s', step (H, V, s) (H', V', s')).
-  Proof.
-    induct 1; simplify; eauto.
-
-    eapply (progress_exp _ _ _ H) in H5; eauto.
     simp.
-    right; do 3 eexists.
-    econstructor.
-    eauto.
-
-    pose proof (progress_exp _ _ _ H _ _ _ _ H3 H4 H5) as Hprog.
-    invert Hprog.
-    assert (Hdropped : eval H1 V e x0).
-    eapply drop_cells; eauto.
-    unfold split in H3; subst.
-    simplify.
-    rewrite lookup_join1; auto.
-    eapply lookup_Some_dom; eauto.
-    pose proof (preservation_exp _ _ _ H _ _ _ H5 Hdropped) as Hpres.
-    simplify.
-    invert Hpres.
-    invert H7; simp.
-    invert H9.
-    apply split_empty_fwd' in H8; subst.
-    invert H11.
-    invert H1.
-    invert H8; simp.
-    invert H9.
-    right; do 3 eexists.
-    econstructor.
-    eauto.
-    eauto.
-    unfold heap1, split in *; subst.
-    rewrite lookup_join1.
-    rewrite lookup_join1.
-    simplify.
-    eauto.
-    eapply lookup_Some_dom; simplify; sets.
-    eapply lookup_Some_dom; simplify.
-    rewrite lookup_join1.
-    simplify; eauto.
-    eapply lookup_Some_dom; simplify; sets.
-
-    pose proof (progress_exp _ _ _ H _ _ _ _ H3 H4 H5) as Hprog.
-    invert Hprog.
-    assert (Hdropped : eval H1 V e x0).
-    eapply drop_cells; eauto.
-    unfold split in H3; subst.
-    simplify.
-    rewrite lookup_join1; auto.
-    eapply lookup_Some_dom; eauto.
-    pose proof (preservation_exp _ _ _ H _ _ _ H5 Hdropped) as Hpres.
-    simplify.
-    invert Hpres.
-    invert H7; simp.
-    invert H9.
-    apply split_empty_fwd' in H8; subst.
-    invert H11.
-    invert H1.
-    invert H8; simp.
-    invert H9.
-    right; do 3 eexists.
-    econstructor.
-    eauto.
-    eauto.
-    unfold heap1, split in *; subst.
-    rewrite lookup_join1.
-    rewrite lookup_join1.
-    simplify.
-    eauto.
-    eapply lookup_Some_dom; simplify; sets.
-    eapply lookup_Some_dom; simplify.
-    rewrite lookup_join1.
-    simplify; eauto.
-    eapply lookup_Some_dom; simplify; sets.
-
-    specialize (IHhoare_triple1 _ _ _ _ H4 H5 H6); simp; eauto 6.
-
-    pose proof (progress_exp _ _ _ H _ _ _ _ H5 H6 H7) as Hprog.
-    invert Hprog.
-    assert (Hdropped : eval H3 V e x).
-    eapply drop_cells; eauto.
-    unfold split in H5; subst.
-    simplify.
-    rewrite lookup_join1; auto.
-    eapply lookup_Some_dom; eauto.
-    pose proof (preservation_exp _ _ _ H _ _ _ H7 Hdropped) as Hpres.
-    simplify.
-    invert Hpres; simp.
-    invert H13.
-    invert H12.
-    cases (weq x2 (^0)); subst; eauto 10.
-
-    pose proof (progress_exp _ _ _ H _ _ _ _ H4 H5 H6) as Hprog.
-    invert Hprog.
-    assert (Hdropped : eval H2 V e x).
-    eapply drop_cells; eauto.
-    unfold split in H4; subst.
-    simplify.
-    rewrite lookup_join1; auto.
-    eapply lookup_Some_dom; eauto.
-    pose proof (preservation_exp _ _ _ H _ _ _ H6 Hdropped) as Hpres.
-    simplify.
-    invert Hpres; simp.
-    invert H12.
-    invert H11.
-    cases (weq x2 (^0)); subst; eauto 10.
-
-    apply H0 in H7.
-    eapply IHhoare_triple in H7; eauto.
-
-    invert H6; simp.
-    eapply IHhoare_triple in H8; eauto.
+    eauto using preservation.
   Qed.
 
-  Theorem hoare_triple_sound : forall P s Q,
-      hoare_triple P s Q
-      -> forall H V, P V H
-      -> invariantFor (trsys_of H V s)
-                      (fun p => (snd p = Skip /\ Q (snd (fst p)) (fst (fst p)))
-                                \/ exists p', step p p').
+  Theorem hoare_triple_sound : forall P {result} (c : cmd result) Q,
+      hoare_triple P c Q
+      -> P $0
+      -> invariantFor (trsys_of $0 c)
+                      (fun p => (exists r, snd p = Return r)
+                                \/ (exists p', step p p')).
+  Proof.
+    simplify.
+
+    eapply invariant_weaken.
+    eapply hoare_triple_sound'; eauto.
+    simp.
+    specialize (progress _ _ _ H1); simplify.
+    specialize (H2 (fst s) (fst s) $0).
+    assert (split (fst s) (fst s) $0) by auto.
+    assert (disjoint (fst s) $0) by auto.
+    cases s; simp; eauto.
+  Qed.
+
+  (* Fancy theorem to help us rewrite within preconditions and postconditions *)
+  Instance hoare_triple_morphism : forall A,
+    Proper (heq ==> eq ==> (eq ==> heq) ==> iff) (@hoare_triple A).
+  Proof.
+    Transparent himp.
+    repeat (hnf; intros).
+    unfold pointwise_relation in *; intuition subst.
+
+    eapply HtConsequence; eauto.
+    rewrite H; reflexivity.
+    intros.
+    hnf in H1.
+    specialize (H1 r _ eq_refl).
+    rewrite H1; reflexivity.
+
+    eapply HtConsequence; eauto.
+    rewrite H; reflexivity.
+    intros.
+    hnf in H1.
+    specialize (H1 r _ eq_refl).
+    rewrite H1; reflexivity.
+    Opaque himp.
+  Qed.
+
+
+  (** * Examples *)
+
+  Global Opaque heq himp lift star exis ptsto.
+
+  Theorem use_lemma : forall result P' (c : cmd result) (Q : result -> hprop) P R,
+    hoare_triple P' c Q
+    -> P ===> P' * R
+    -> hoare_triple P c (fun r => Q r * R)%sep.
+  Proof.
+    simp.
+    eapply HtWeaken.
+    eapply HtFrame.
+    eassumption.
+    eauto.
+  Qed.
+
+  Theorem HtRead' : forall a v,
+    hoare_triple (a |-> v)%sep (Read a) (fun r => a |-> v * [| r = v |])%sep.
+  Proof.
+    simp.
+    apply HtWeaken with (exists r, a |-> r * [| r = v |])%sep.
+    eapply HtStrengthen.
+    apply HtRead.
+    simp.
+    cancel; auto.
+    subst; cancel.
+    cancel; auto.
+  Qed.
+
+  Theorem HtRead'' : forall p P R,
+    P ===> (exists v, p |-> v * R v)
+    -> hoare_triple P (Read p) (fun r => p |-> r * R r)%sep.
+  Proof.
+    simp.
+    eapply HtWeaken.
+    apply HtRead.
+    assumption.
+  Qed.
+
+  Ltac basic := apply HtReturn' || eapply HtWrite.
+
+  Ltac step0 := basic || eapply HtBind || (eapply use_lemma; [ basic | cancel; auto ])
+                || (eapply use_lemma; [ eapply HtRead' | solve [ cancel; auto ] ])
+                || (eapply HtRead''; solve [ cancel ])
+                || (eapply HtStrengthen; [ eapply use_lemma; [ basic | cancel; auto ] | ])
+                || (eapply HtConsequence; [ apply HtFail | .. ]).
+  Ltac step := step0; simp.
+  Ltac ht := simp; repeat step.
+  Ltac conseq := simplify; eapply HtConsequence.
+  Ltac use_IH H := conseq; [ apply H | .. ]; ht.
+  Ltac loop_inv0 Inv := (eapply HtWeaken; [ apply HtLoop with (I := Inv) | .. ])
+                        || (eapply HtConsequence; [ apply HtLoop with (I := Inv) | .. ]).
+  Ltac loop_inv Inv := loop_inv0 Inv; ht.
+  Ltac use H := (eapply use_lemma; [ eapply H | cancel; auto ])
+                || (eapply HtStrengthen; [ eapply use_lemma; [ eapply H | cancel; auto ] | ]).
+
+  Ltac heq := intros; apply himp_heq; split.
+
+
+  (** * List-reverse example *)
+
+  Fixpoint linkedList (p : wrd) (ls : list wrd) :=
+    match ls with
+      | nil => [| p = ^0 |]
+      | x :: ls' => [| p <> ^0 |]
+                    * exists p', p |--> [x; p'] * linkedList p' ls'
+    end%sep.
+
+  Theorem linkedList_null : forall ls,
+    linkedList (^0) ls === [| ls = nil |].
+  Proof.
+    heq; cases ls; cancel.
+  Qed.
+
+  Theorem linkedList_nonnull : forall p ls,
+    p <> ^0
+    -> linkedList p ls === exists x ls' p', [| ls = x :: ls' |] * p |--> [x; p'] * linkedList p' ls'.
+  Proof.
+    heq; cases ls; cancel; match goal with
+                           | [ H : _ = _ :: _ |- _ ] => invert H
+                           end; cancel.
+  Qed.
+
+  Hint Rewrite <- rev_alt.
+  Hint Rewrite rev_involutive.
+
+  Opaque linkedList.
+
+  Definition reverse p :=
+    pr <- for pr := (p, ^0) loop
+      let (p, r) := pr in
+      if weq p (^0) then
+        Return (Done pr)
+      else
+        tmp <- Read (p ^+ ^1);
+        _ <- Write (p ^+ ^1) r;
+        Return (Again (tmp, p))
+    done;
+    Return (snd pr).
+
+  Definition valueOf {A} (o : loop_outcome A) :=
+    match o with
+    | Done v => v
+    | Again v => v
+    end.
+
+  Theorem reverse_ok : forall p ls,
+    {{linkedList p ls}}
+      reverse p
+    {{r ~> linkedList r (rev ls)}}.
+  Proof.
+    unfold reverse.
+    simp.
+    step.
+    loop_inv (fun o => exists ls1 ls2, [| ls = rev_append ls1 ls2 |]
+                                       * linkedList (fst (valueOf o)) ls2
+                                       * linkedList (snd (valueOf o)) ls1
+                                       * [| match o with
+                                            | Done (p, _) => p = ^0
+                                            | _ => True
+                                            end |])%sep.
+    cases (weq a (^0)); simp.
+    step.
+    cancel.
+    step.
+    setoid_rewrite (linkedList_nonnull _ _ n).
+    step.
+    simp.
+    step.
+    step.
+    simp.
+    step.
+    setoid_rewrite (linkedList_nonnull _ _ n).
+    cancel.
+    simp.
+    setoid_rewrite linkedList_null.
+    cancel.
+    equality.
+    simp.
+    step.
+    cancel.
+    simp.
+    setoid_rewrite linkedList_null.
+    cancel.
+    simp.
+    cancel.
+  Qed.
+
+  Opaque reverse.
+End MixedEmbedded.
+
+
+(** * A simple C-like language with just two data types *)
+
+Module DeeplyEmbedded(Import BW : BIT_WIDTH).
+  Definition wrd := word bit_width.
+
+  Inductive exp :=
+  | Var (x : var)
+  | Const (n : wrd)
+  | Add (e1 e2 : exp)
+  | Head (e : exp)
+  | Tail (e : exp)
+  | NotNull (e : exp).
+
+  Inductive stmt :=
+  | Skip
+  | Assign (x : var) (e : exp)
+  | WriteHead (x : var) (e : exp)
+  | WriteTail (x : var) (e : exp)
+  | Seq (s1 s2 : stmt)
+  | IfThenElse (e : exp) (s1 s2 : stmt)
+  | WhileLoop (e : exp) (s1 : stmt).
+
+  Inductive type :=
+  | Scalar
+  | ListPointer (t : type).
+
+  Definition type_eq : forall t1 t2 : type, sumbool (t1 = t2) (t1 <> t2).
+    decide equality.
+  Defined.
+
+  Record function := {
+    Params : list (var * type);
+    Locals : list (var * type);
+    Return : type;
+    Body : stmt
+  }.
+
+  Section fn.
+    Variable fn : function.
+
+    Definition vars := Params fn ++ Locals fn ++ [("result", Return fn)].
+
+    Fixpoint varType (x : var) (vs : list (var * type)) : option type :=
+      match vs with
+      | nil => None
+      | (y, t) :: vs' => if y ==v x then Some t else varType x vs'
+      end.
+
+    Fixpoint expType (e : exp) : option type :=
+      match e with
+      | Var x => varType x vars
+      | Const _ => Some Scalar
+      | Add e1 e2 => match expType e1, expType e2 with
+                     | Some Scalar, Some Scalar => Some Scalar
+                     | _, _ => None
+                     end
+      | Head x => match expType x with
+                  | Some (ListPointer t) => Some t
+                  | _ => None
+                  end
+      | Tail x => match expType x with
+                  | Some (ListPointer t) => Some (ListPointer t)
+                  | _ => None
+                  end
+      | NotNull e1 => match expType e1 with
+                      | Some (ListPointer _) => Some Scalar
+                      | _ => None
+                      end
+      end.
+
+    Fixpoint stmtWf (s : stmt) : bool :=
+      match s with
+      | Skip => true
+      | Assign x e => match varType x vars, expType e with
+                      | Some t1, Some t2 =>
+                        if type_eq t1 t2 then true else false
+                      | _, _ => false
+                      end
+      | WriteHead x e => match varType x vars, expType e with
+                         | Some (ListPointer t1), Some t2 =>
+                           if type_eq t1 t2 then true else false
+                         | _, _ => false
+                         end
+      | WriteTail x e => match varType x vars, expType e with
+                         | Some (ListPointer t1), Some (ListPointer t2) =>
+                           if type_eq t1 t2 then true else false
+                         | _, _ => false
+                         end
+      | Seq s1 s2 => stmtWf s1 && stmtWf s2
+      | IfThenElse e s1 s2 => match expType e with
+                              | Some Scalar => stmtWf s1 && stmtWf s2
+                              | _ => false
+                              end
+      | WhileLoop e s1 => match expType e with
+                          | Some Scalar => stmtWf s1
+                          | _ => false
+                          end
+      end.
+
+    Record functionWf : Prop := {
+      VarsOk : NoDup (map fst (Params fn ++ Locals fn));
+      BodyOk : stmtWf (Body fn) = true
+    }.
+  End fn.
+
+  Definition heap := fmap (wrd) (wrd * wrd).
+  Definition valuation := fmap var wrd.
+
+  Inductive eval : heap -> valuation -> exp -> wrd -> Prop :=
+  | VVar : forall H V x v,
+      V $? x = Some v
+      -> eval H V (Var x) v
+  | VConst : forall H V n,
+      eval H V (Const n) n
+  | VAdd : forall H V e1 e2 n1 n2,
+      eval H V e1 n1
+      -> eval H V e2 n2
+      -> eval H V (Add e1 e2) (n1 ^+ n2)
+  | VHead : forall H V e1 p ph pt,
+      eval H V e1 p
+      -> H $? p = Some (ph, pt)
+      -> eval H V (Head e1) ph
+  | VTail : forall H V e1 p ph pt,
+      eval H V e1 p
+      -> H $? p = Some (ph, pt)
+      -> eval H V (Tail e1) pt
+  | VNotNull : forall H V e1 p,
+      eval H V e1 p
+      -> eval H V (NotNull e1) (if weq p (^0) then ^1 else ^0).
+
+  Inductive step : heap * valuation * stmt -> heap * valuation * stmt -> Prop :=
+  | StAssign : forall H V x e v,
+      eval H V e v
+      -> step (H, V, Assign x e) (H, V $+ (x, v), Skip)
+  | StWriteHead : forall H V x e a v hv tv,
+      V $? x = Some a
+      -> eval H V e v
+      -> H $? a = Some (hv, tv)
+      -> step (H, V, WriteHead x e) (H $+ (a, (v, tv)), V, Skip)
+  | StWriteTail : forall H V x e a v hv tv,
+      V $? x = Some a
+      -> eval H V e v
+      -> H $? a = Some (hv, tv)
+      -> step (H, V, WriteTail x e) (H $+ (a, (hv, v)), V, Skip)
+  | StSeq1 : forall H V s2,
+      step (H, V, Seq Skip s2) (H, V, s2)
+  | StSeq2 : forall H V s1 s2 H' V' s1',
+      step (H, V, s1) (H', V', s1')
+      -> step (H, V, Seq s1 s2) (H', V', Seq s1' s2)
+  | StIfThen : forall H V e s1 s2 n,
+      eval H V e n
+      -> n <> ^0
+      -> step (H, V, IfThenElse e s1 s2) (H, V, s1)
+  | StIfElse : forall H V e s1 s2,
+      eval H V e (^0)
+      -> step (H, V, IfThenElse e s1 s2) (H, V, s2)
+  | StWhileTrue : forall H V e s1 n,
+      eval H V e n
+      -> n <> ^0
+      -> step (H, V, WhileLoop e s1) (H, V, Seq s1 (WhileLoop e s1))
+  | StWhileFalse : forall H V e s1,
+      eval H V e (^0)
+      -> step (H, V, WhileLoop e s1) (H, V, Skip).
+
+  Definition trsys_of (H : heap) (V : valuation) (s : stmt) := {|
+    Initial := {(H, V, s)};
+    Step := step
+  |}.
+End DeeplyEmbedded.
+
+
+(** * Connecting the two *)
+
+Module MixedToDeep(Import BW : BIT_WIDTH).
+  Module Import DE := DeeplyEmbedded(BW).
+  Module Import ME := MixedEmbedded(BW).
+
+  Inductive translate_exp (V : valuation) : forall {A}, A -> exp -> Prop :=
+  | TrAdd : forall (v1 v2 : wrd) e1 e2,
+      translate_exp V v1 e1
+      -> translate_exp V v2 e2
+      -> translate_exp V (v1 ^+ v2) (Add e1 e2)
+  | TrVar : forall x v,
+      V $? x = Some v
+      -> translate_exp V v (Var x)
+  | TrConst : forall v,
+      translate_exp V v (Const v).
+
+  Fixpoint couldWrite (x : var) (s : stmt) : bool :=
+    match s with
+    | Assign y _ => if x ==v y then true else false
+    | Skip
+    | WriteHead _ _
+    | WriteTail _ _ => false
+    | Seq s1 s2
+    | IfThenElse _ s1 s2 => couldWrite x s1 || couldWrite x s2
+    | WhileLoop _ s1 => couldWrite x s1
+    end.
+
+  Inductive translate (out : var) : valuation -> forall {A}, cmd A -> stmt -> Prop :=
+  | TrReturn : forall V (A : Set) (v : A) e,
+      translate_exp V v e
+      -> translate out V (Return v) (Assign out e)
+  | TrReturned : forall V v,
+      V $? out = Some v
+      -> translate out V (Return v) Skip
+  | TrAssign : forall V (B : Set) (v : wrd) (c : wrd -> cmd B) e x s1,
+      translate_exp V v e
+      -> (forall w, translate out (V $+ (x, w)) (c w) s1)
+      -> translate out V (Bind (Return v) c) (Seq (Assign x e) s1)
+  | TrAssigned : forall V (B : Set) (v : wrd) (c : wrd -> cmd B) x s1,
+      V $? x = Some v
+      -> translate out (V $+ (x, v)) (c v) s1
+      -> translate out V (Bind (Return v) c) (Seq Skip s1).
+
+  Example adder (a b c : wrd) :=
+    Bind (Return (a ^+ b)) (fun ab => Return (ab ^+ c)).
+
+  Ltac freshFor vm k :=
+    let rec keepTrying x :=
+        let H := fresh in
+        (assert (H : vm $? x = None) by (simplify; equality);
+         clear H; k x)
+        || let x' := eval simpl in (x ++ "'")%string in keepTrying x' in
+    keepTrying "tmp".
+
+  Ltac translate :=
+    match goal with
+    | [ |- translate_exp _ (_ ^+ _) _ ] => eapply TrAdd
+    | [ |- translate_exp ?V ?v _ ] =>
+      match V with
+      | context[add _ ?y v] => apply TrVar with (x := y); simplify; equality
+      end
+
+    | [ |- translate _ _ (Return _) _ ] => apply TrReturn
+    | [ |- translate _ ?V (Bind (Return _) _) _ ] =>
+      freshFor V ltac:(fun y =>
+                         eapply TrAssign with (x := y); [ | intro ])
+    end.
+
+  Lemma translate_adder : sig (fun s =>
+        forall a b c, translate "result" ($0 $+ ("a", a) $+ ("b", b) $+ ("c", c)) (adder a b c) s).
+  Proof.
+    eexists; simplify.
+    unfold adder.
+    repeat translate.
+  Defined.
+
+  Definition adder_compiled := Eval simpl in proj1_sig translate_adder.
+
+  Inductive translated : forall {A}, DE.heap * valuation * stmt -> ME.heap * cmd A -> Prop :=
+  | Translated : forall A H h V s (c : cmd A),
+      translate "result" V c s
+      -> translated (H, V, s) (h, c).
+
+  Lemma eval_translate : forall H V e v,
+      eval H V e v
+      -> forall (v' : wrd), translate_exp V v' e
+      -> v = v'.
+  Proof.
+    induct 1; invert 1; simplify.
+
+    apply inj_pair2 in H2; subst.
+    equality.
+
+    apply inj_pair2 in H1; subst.
+    equality.
+
+    apply inj_pair2 in H1; subst.
+    erewrite IHeval1 by eauto.
+    erewrite IHeval2 by eauto.
+    equality.
+  Qed.
+
+  Lemma multistep_bind : forall A h (c1 : cmd A) h' c1',
+      step^* (h, c1) (h', c1')
+      -> forall B (c2 : A -> cmd B), step^* (h, Bind c1 c2) (h', Bind c1' c2).
+  Proof.
+    induct 1; eauto.
+    cases y; simplify.
+    specialize (IHtrc _ _ _ _ _ eq_refl JMeq.JMeq_refl JMeq.JMeq_refl JMeq.JMeq_refl _ c2).
+    eauto.
+  Qed.
+
+  Lemma step_translate : forall H V s H' V' s',
+      DE.step (H, V, s) (H', V', s')
+      -> forall h (c : cmd wrd) out,
+        translate out V c s
+        -> exists c', ME.step^* (h, c) (h, c')
+                      /\ translate out V' c' s'.
+  Proof.
+    induct 1; invert 1; simplify.
+
+    apply inj_pair2 in H1; subst.
+    eapply eval_translate in H5; eauto; subst.
+    eexists; propositional.
+    eauto.
+    apply TrReturned; simplify; auto.
+
+    apply inj_pair2 in H0; subst.
+    eexists; propositional.
+    eapply TrcFront.
+    eauto.
+    eauto.
+    replace V' with (V' $+ (x, v)).
+    assumption.
+    maps_equal.
+    symmetry; assumption.
+
+    apply inj_pair2 in H2; subst.
+    invert H0.
+    eexists; propositional.
+    eauto.
+    eapply TrAssigned with (x := x).
+    eapply eval_translate in H7; eauto.
+    simplify.
+    subst.
+    reflexivity.
+    match goal with
+    | [ |- translate _ ?V' _ _ ] => replace V' with (V $+ (x, v)) by (maps_equal; equality)
+    end.
+    eauto.
+
+    invert H0.
+  Qed.
+
+  Theorem translated_simulates : forall H V c h s,
+      translate "result" V c s
+      -> simulates (translated (A := wrd)) (DE.trsys_of H V s) (ME.multistep_trsys_of h c).
+  Proof.
+    constructor; simplify.
+
+    propositional; subst.
+    eexists; split.
+    econstructor.
+    eassumption.
+    eauto.
+
+    invert H1.
+    apply inj_pair2 in H4; subst.
+    cases st1'.
+    cases p.
+    eapply step_translate in H2; eauto.
+    first_order.
+    eexists; split; [ | eassumption ].
+    econstructor.
+    assumption.
+  Qed.
+
+  Hint Constructors eval DE.step.
+
+  Lemma translate_exp_sound : forall V v e,
+      translate_exp V v e
+      -> forall H, eval H V e v.
+  Proof.
+    induct 1; simplify; eauto.
+  Qed.
+
+  Hint Resolve translate_exp_sound.
+
+  Lemma not_stuck : forall A h (c : cmd A) h' c',
+      step (h, c) (h', c')
+      -> forall out V s, translate out V c s
+                         -> forall H, exists p', DE.step (H, V, s) p'.
+  Proof.
+    induct 1; invert 1; simplify.
+
+    eexists.
+    econstructor.
+    econstructor.
+    eauto.
+
+    eexists.
+    econstructor.
+
+    eexists.
+    econstructor.
+    econstructor.
+    eauto.
+
+    eexists.
+    econstructor.
+  Qed.
+
+  Theorem hoare_triple_sound : forall P (c : cmd wrd) Q V s,
+      hoare_triple P c Q
+      -> P $0
+      -> translate "result" V c s
+      -> V $? "result" = None
+      -> invariantFor (DE.trsys_of $0 V s)
+                      (fun p => snd p = Skip
+                                \/ exists p', DE.step p p').
   Proof.
     simplify.
     eapply invariant_weaken.
-    eapply hoare_triple_sound'; eauto.
-    simplify.
+    eapply invariant_simulates.
+    apply translated_simulates.
+    eassumption.
+    apply invariant_multistepify with (sys := trsys_of $0 c).
+    eauto using hoare_triple_sound.
+    invert 1; first_order.
 
-    cases s0.
-    cases p.
-    simplify.
-    pose proof (progress _ _ _ H2 v h h $0) as Hprog; simplify.
-    cases Hprog; eauto.
-    subst.
-    eapply invert_Skip in H2.
-    left; propositional.
-    apply H2; auto.
-    first_order.
+    cases st2; simplify; subst.
+    invert H4; simplify.
+    apply inj_pair2 in H9; subst.
+    invert H8.
+    apply inj_pair2 in H4; subst.
+    right; eexists.
+    econstructor; eauto.
+    auto.
+
+    invert H4.
+    apply inj_pair2 in H6; subst; simplify.
+    cases x.
+    eapply not_stuck in H3; eauto.
   Qed.
 
-End DeeplyEmbedded.
+  Theorem adder_ok : forall a b c,
+      {{emp}}
+        adder a b c
+      {{r ~> [| r = a ^+ b ^+ c |]}}.
+  Proof.
+    unfold adder.
+    simplify.
+    step.
+    step.
+    instantiate (1 := (fun r => [| r = a ^+ b |])%sep).
+    cancel.
+    simp.
+    step.
+    cancel.
+    equality.
+  Qed.
+
+  Theorem adder_compiled_ok : forall a b c,
+      invariantFor (DE.trsys_of $0 ($0 $+ ("a", a) $+ ("b", b) $+ ("c", c)) adder_compiled)
+                      (fun p => snd p = Skip
+                                \/ exists p', DE.step p p').
+  Proof.
+    simplify.
+    eapply hoare_triple_sound.
+    apply adder_ok.
+    constructor; auto.
+    apply (proj2_sig translate_adder).
+    simplify; equality.
+  Qed.
+End MixedToDeep.
+
+
+(** * Getting concrete *)
+
+Module Bw64.
+  Definition bit_width := 64.
+  Theorem bit_width_nonzero : bit_width > 0.
+  Proof.
+    unfold bit_width; linear_arithmetic.
+  Qed.
+End Bw64.
+
+Module MixedEmbedded64.
+  Module Import ME := MixedEmbedded(Bw64).
+End MixedEmbedded64.
